\documentclass[journal,12pt,twocolumn]{IEEEtran}

\usepackage{setspace}
\usepackage{gensymb}
\singlespacing
\usepackage[cmex10]{amsmath}

\usepackage{amsthm}

\usepackage{mathrsfs}
\usepackage{txfonts}
\usepackage{stfloats}
\usepackage{bm}
\usepackage{cite}
\usepackage{cases}
\usepackage{subfig}

\usepackage{longtable}
\usepackage{multirow}

\usepackage{enumitem}
\usepackage{mathtools}
\usepackage{steinmetz}
\usepackage{tikz}
\usepackage{circuitikz}
\usepackage{verbatim}
\usepackage{tfrupee}
\usepackage[breaklinks=true]{hyperref}
\usepackage{graphicx}
\usepackage{tkz-euclide}

\usetikzlibrary{calc,math}
\usepackage{listings}
    \usepackage{color}                                            %%
    \usepackage{array}                                            %%
    \usepackage{longtable}                                        %%
    \usepackage{calc}                                             %%
    \usepackage{multirow}                                         %%
    \usepackage{hhline}                                           %%
    \usepackage{ifthen}                                           %%
    \usepackage{lscape}     
\usepackage{multicol}
\usepackage{chngcntr}

\DeclareMathOperator*{\Res}{Res}

\renewcommand\thesection{\arabic{section}}
\renewcommand\thesubsection{\thesection.\arabic{subsection}}
\renewcommand\thesubsubsection{\thesubsection.\arabic{subsubsection}}

\renewcommand\thesectiondis{\arabic{section}}
\renewcommand\thesubsectiondis{\thesectiondis.\arabic{subsection}}
\renewcommand\thesubsubsectiondis{\thesubsectiondis.\arabic{subsubsection}}


\hyphenation{op-tical net-works semi-conduc-tor}
\def\inputGnumericTable{}                                 %%

\lstset{
%language=C,
frame=single, 
breaklines=true,
columns=fullflexible
}
\begin{document}


\newtheorem{theorem}{Theorem}[section]
\newtheorem{problem}{Problem}
\newtheorem{proposition}{Proposition}[section]
\newtheorem{lemma}{Lemma}[section]
\newtheorem{corollary}[theorem]{Corollary}
\newtheorem{example}{Example}[section]
\newtheorem{definition}[problem]{Definition}

\newcommand{\BEQA}{\begin{eqnarray}}
\newcommand{\EEQA}{\end{eqnarray}}
\newcommand{\define}{\stackrel{\triangle}{=}}
\bibliographystyle{IEEEtran}
\raggedbottom
\setlength{\parindent}{0pt}
\providecommand{\mbf}{\mathbf}
\providecommand{\pr}[1]{\ensuremath{\Pr\left(#1\right)}}
\providecommand{\qfunc}[1]{\ensuremath{Q\left(#1\right)}}
\providecommand{\sbrak}[1]{\ensuremath{{}\left[#1\right]}}
\providecommand{\lsbrak}[1]{\ensuremath{{}\left[#1\right.}}
\providecommand{\rsbrak}[1]{\ensuremath{{}\left.#1\right]}}
\providecommand{\brak}[1]{\ensuremath{\left(#1\right)}}
\providecommand{\lbrak}[1]{\ensuremath{\left(#1\right.}}
\providecommand{\rbrak}[1]{\ensuremath{\left.#1\right)}}
\providecommand{\cbrak}[1]{\ensuremath{\left\{#1\right\}}}
\providecommand{\lcbrak}[1]{\ensuremath{\left\{#1\right.}}
\providecommand{\rcbrak}[1]{\ensuremath{\left.#1\right\}}}
\theoremstyle{remark}
\newtheorem{rem}{Remark}
\newcommand{\sgn}{\mathop{\mathrm{sgn}}}
%\providecommand{\abs}[1]{\left\vert#1\right\vert}
\providecommand{\res}[1]{\Res\displaylimits_{#1}} 
%\providecommand{\norm}[1]{\left\lVert#1\right\rVert}
\providecommand{\norm}[1]{\lVert#1\rVert}
\providecommand{\mtx}[1]{\mathbf{#1}}
%\providecommand{\mean}[1]{E\left[ #1 \right]}
\providecommand{\fourier}{\overset{\mathcal{F}}{ \rightleftharpoons}}
%\providecommand{\hilbert}{\overset{\mathcal{H}}{ \rightleftharpoons}}
\providecommand{\system}{\overset{\mathcal{H}}{ \longleftrightarrow}}
	%\newcommand{\solution}[2]{\textbf{Solution:}{#1}}
\newcommand{\solution}{\noindent \textbf{Solution: }}
\newcommand{\cosec}{\,\text{cosec}\,}
\providecommand{\dec}[2]{\ensuremath{\overset{#1}{\underset{#2}{\gtrless}}}}
\newcommand{\myvec}[1]{\ensuremath{\begin{pmatrix}#1\end{pmatrix}}}
\newcommand{\mydet}[1]{\ensuremath{\begin{vmatrix}#1\end{vmatrix}}}
\numberwithin{equation}{subsection}
\makeatletter
\@addtoreset{figure}{problem}
\makeatother
\let\StandardTheFigure\thefigure
\let\vec\mathbf
\renewcommand{\thefigure}{\theproblem}
\def\putbox#1#2#3{\makebox[0in][l]{\makebox[#1][l]{}\raisebox{\baselineskip}[0in][0in]{\raisebox{#2}[0in][0in]{#3}}}}
     \def\rightbox#1{\makebox[0in][r]{#1}}
     \def\centbox#1{\makebox[0in]{#1}}
     \def\topbox#1{\raisebox{-\baselineskip}[0in][0in]{#1}}
     \def\midbox#1{\raisebox{-0.5\baselineskip}[0in][0in]{#1}}
\vspace{3cm}
\title{EE3025 - Assignment 1}
\author{Ch Pranay Prakash - EE18BTECH11009}
\maketitle
\newpage
\bigskip
\renewcommand{\thefigure}{\theenumi}
\renewcommand{\thetable}{\theenumi}
Download all python codes from 
\begin{lstlisting}
https://github.com/pranayEE11009/EE3025_IDP/tree/main/Assignment_1/codes
\end{lstlisting}
%
and latex-tikz codes from 
%
\begin{lstlisting}
https://github.com/pranayEE11009/EE3025_IDP/tree/main/Assignment_1
\end{lstlisting}
\section{Problem}
\begin{enumerate}[label=\thesection.\arabic*.,ref=\thesection.\theenumi]
\numberwithin{equation}{enumi}
\item
Let
\begin{align}
    x(n) = \cbrak{\underset{\uparrow}{1},2,3,4,2,1} 
\end{align}
and 
\begin{multline}
    y(n) + \frac{1}{2}y(n-1) = x(n) + x(n-2) \label{eq:1.0.2}
    \\
    y(n) = 0 , n<0
\end{multline}

Compute
\begin{align}
    X(k) = \sum_{n=0}^{N-1}x(n)e^{-j2\pi kn/N},
    \quad k=0,1, \ldots, N-1
\end{align}

and H(k) using h(n).\\
\end{enumerate}

\section{Solution}
\begin{enumerate}[label=\thesection.\arabic*.,ref=\thesection.\theenumi]
\numberwithin{equation}{enumi}
\item
Since, We know that the Impulse response of an LTI system is the output of the system
when an Unit Impulse signal is given as the input to the system.\\

Now, from  equation \eqref{eq:1.0.2} the impulse response of the system can be defined as,
\begin{align}
    h(n) + \frac{1}{2}h(n-1) = \delta(n) + \delta(n-2)	
    \\
    \implies h(n) = \delta(n) + \delta(n-2) - \frac{1}{2}h(n-1) \label{eq:hn}
\end{align}

\item
{ \bf Computing the DFT manually:} 

The DFT of the Input Signal x(n) is given \\
by :
\begin{align}
    X(k) = \sum_{n=0}^{N-1}x(n)e^{-j2\pi kn/N},\quad k=0,1, \ldots, N-1 
\end{align}

Similarly, the DFT of the Impulse Response h(n) is given by :
\begin{align}
    H(k) = \sum_{n=0}^{N-1}h(n)e^{-j2\pi kn/N},\quad k=0,1, \ldots, N-1 
\end{align}
The following python code computes the DFT of x(n) and h(n).
\begin{lstlisting}
https://github.com/pranayEE11009/EE3025_IDP/blob/main/Assignment_1/codes/ee18btech11009.py
\end{lstlisting}
The plots are in
\begin{lstlisting}
https://github.com/pranayEE11009/EE3025_IDP/tree/main/Assignment_1/figs
\end{lstlisting}
%%%%%%%%%%%%%%%%%%%%%%%%%%%%%%%%%%%%%%%%%%%%%%%%%%%%%%%%%%%%%%%%%%%%%%%%%%%%%%%%%5

\newpage

\begin{figure}[h!]
    \centering
    \includegraphics[height=6.8cm,width=9cm]{x.png}
    \label{figs}
\end{figure}

\begin{figure}[h!]
    \centering
    \includegraphics[height=6.8cm,width=9cm]{Xamp.png}
    \label{figs}
\end{figure}

\begin{figure}[h!]
    \centering
    \includegraphics[height=6.8cm,width=9.25cm]{Hamp.png}
    \label{figs}
\end{figure}

\begin{figure}[h!]
    \centering
    \includegraphics[height=6.8cm,width=9cm]{h.png}
    \label{figs}
\end{figure}
\vspace{1cm}
\begin{figure}[h!]
    \centering
    \includegraphics[height=6.8cm,width=9.5cm]{Xpha.png}
    \label{figs}
\end{figure}

\begin{figure}[h!]
    \centering
    \includegraphics[height=6.8cm,width=9.5cm]{Hpha.png}
    \label{figs}
\end{figure}

%%%%%%%%%%%%%%%%%%%%%%%%%%%%%%%%%%%%%%%%%%%%%%%%%%%%%%%%%%%%%%%%%%%%%%%%%%%%%%%

\newpage
\item
{ \bf Computing the DFT manually using matrix multiplication:} \\

We know that DFT of x(n) is, \\
\begin{align}
    X(k) \triangleq \sum_{n=0}^{N-1}x(n)e^{-j2\pi kn/N},\quad k=0,1, \ldots, N-1 
\end{align}

Let us define a matrix ''W'', a NxN matrix, such that, 
\begin{align}
    DFT(x)= X = W.x  \label{eq:dftx}
\end{align}
\emph {Where (.) represents the matrix multiplication of W and x.} \\
Each point of the matrix W is defined as, \\
\begin{align}
    W_N^{nk}=e^{-j2\pi kn/N} \\
\end{align}
\emph{where n and k are column and row indices of the matrix respectively.} \\

Now from equation: \eqref{eq:dftx}, DFT(x) using the DFT matrix is given by,
\begin{equation}
 \begin{bmatrix} X(0) \\ X(1) \\ X(2) \\ \vdots \\ X(N-1) \end{bmatrix}
=
\begin{bmatrix}
1 & 1 & \cdots & 1 \\
1 & W_N^1& \cdots & W_N^{N-1}\\
1 & W_N^2 & \cdots & W_N^{2(N-1)}\\
\vdots & \vdots & \ddots & \vdots \\
1 & W_N^{N-1} & \cdots &W_N^{(N-1)(N-1)}
\end{bmatrix}
\begin{bmatrix}
x(0) \\ x(1) \\ x(2) \\ \vdots \\x(N-1)
\end{bmatrix}
\end{equation}
\bigskip

Given,  x(n) = \cbrak{\underset{\uparrow}{1},2,3,4,2,1} and N=6\\
we have,
\begin{equation}
\begin{bmatrix} X(0) \\ X(1) \\ X(2) \\ X(3) \\ X(4) \\ X(5) \end{bmatrix}
=
\begin{bmatrix}
1 +2+3+4+2+1 \\ 1+ (2)e^{-j\pi /3} + ... + (1)e^{-j5\pi /3}\\ 1 + (2)e^{-2j\pi /3} + ... +(1)(e^{-2j5\pi /3}\\ 1 + (2)e^{-3j\pi /3} + ... + (1)e^{-3j5\pi /3}\\ 1 + (2)e^{-4j\pi /3} + ... + (1)e^{-4j5\pi /3}\\ 1 + (2)e^{-5j\pi /3} + ... + (1)e^{-5j5\pi /3}
\end{bmatrix}
\end{equation}
\bigskip

On Solving we get,
\begin{align}
    X(0)= 13 + 0j \\
    X(1)= -4 - 1.732j \\
    X(2)= 1 + 0j \\
    X(3)= -1 + 0j \\
    X(4)= 1 + 0j \\
    X(5)= -4 + 1.732j
\end{align}
We can observe that these values are same as the values that we obtained from the plots.
\bigskip


Similarly, the DFT of h(n) can be defined as,
\begin{align}
    DFT(h)= H = W.h  \label{eq:dfth}
\end{align}

So, we have,
\begin{equation}
 \begin{bmatrix} H(0) \\ H(1) \\ H(2) \\ \vdots \\ H(N-1) \end{bmatrix}
=
\begin{bmatrix}
1 & 1 & \cdots & 1 \\
1 & W_N^1& \cdots & W_N^{N-1}\\
1 & W_N^2 &\cdots & W_N^{2(N-1)}\\
\vdots & \vdots & \ddots & \vdots\\
1 & W_N^{N-1} & \cdots &W_N^{(N-1)(N-1)}
\end{bmatrix}
\begin{bmatrix}
h(0) \\ h(1) \\ h(2) \\ \vdots \\ h(N-1)
\end{bmatrix}
\end{equation}

\begin{equation}
\begin{bmatrix} H(0) \\ H(1) \\ H(2) \\ H(3) \\ H(4) \\ H(5) \end{bmatrix}
=
\begin{bmatrix}
h(0) + h(1) + h(2) + h(3) + h(4) + h(5) \\h(0) + h(1)e^{-j\pi /3} + ... + h(5)e^{-j5\pi /3}\\h(0) + h(1)e^{-2j\pi /3} + ... + h(5)e^{-2j5\pi /3}\\h(0) + h(1)e^{-3j\pi /3} + ... + h(5)e^{-3j5\pi /3}\\
h(0) + h(1)e^{-4j\pi /3} + ... + h(5)e^{-4j5\pi /3}\\h(0) + h(1)e^{-5j\pi /3} + ... + h(5)e^{-5j5\pi /3}
\end{bmatrix}
\end{equation}
\bigskip

Now, from equation: \eqref{eq:hn} we know that,
\begin{align}
     h(n) = \delta(n) + \delta(n-2) - \frac{1}{2}h(n-1) 
\end{align}
for N=6,
\begin{align}
     h(n) = \cbrak{\underset{\uparrow}{1},-0.5,1.25,-0.625,0.3125,-0.15625} 
\end{align}

Therefore, on solving we get,
\begin{align}
    H(0) = 1.28125 + 0j,\\
    H(1) = 0.515625 - 0.5142026j,\\
    H(2) = -0.078125 + 1.109595j,\\
    H(3) = 3.84375 + 0j,\\
    H(4) = -0.078125 - 1.109595j.\\
    H(5) = 0.515625 + 0.51420256j
\end{align}
We can observe that these values are same as the values that we obtained from the plots.

\end{enumerate}


%%%%%%%%%%%%%%%%-- FFT ALGORITHM 

\section {{8-point FFT}}
\begin{enumerate}[label=\thesection.\arabic*.,ref=\thesection.\theenumi]
\numberwithin{equation}{enumi}
\item
{\bf{N-point FFT Algorithm:}}

The N-point DFT of a signal $x(n)$ is,
\begin{align}
    X(k) = \sum_{n=0}^{N-1}x(n)e^{-j2\pi kn/N},
    \quad k=0,1, \ldots, N-1 \label{eq:3dftx}
\end{align}

Let $F_N$ be a N-point DFT matrix, then the DFT of $x(n)$ in the matrix form is given by,
\begin{align}
    X(k) = {F_{N}}.x(n)
\end{align}

For the ease of calculation eq\eqref{eq:3dftx} can be broken down into two terms.
Even-indexed n term and odd-indexed n term.
\begin{align}
    X(k) &= \sum_{n=0(even-n)}^{N-1} x(n)W^{kn}_{N} + \sum_{n=0(odd-n)}^{N-1} x(n)W^{kn}_{N} \\
    &= \sum_{m=0}^{N/2 -1} x(2m)W^{2mk}_{N} + \sum_{m=0}^{N/2 -1} x(2m+1)W^{(2m+1)k}_{N} \\
    &= \sum_{m=0}^{N/2 -1} x(2m)W^{2mk}_{N} + W^{k}_{N} \sum_{m=0}^{N/2 -1} x(2m+1)W^{2mk}_{N} \label{eq:3.1.5}
\end{align}

$\because$ complex exponential, $W_{N}^{nk}$ exhibits the following property,

\begin{align}
   (i) \quad W^{2}_{N} = W_{N/2}
\end{align}
\begin{align}
    [ \because (e^{-j2\pi kn/N})^2 = e^{-j2\pi kn/{(N/2)}}]
\end{align}
 using this property eq\eqref{eq:3.1.5} can be written as,

\begin{align}
    X(k) = \sum_{m=0}^{{N/2}-1} x(2m)W^{km}_{N/2} +W^{k}_{N} \sum_{m=0}^{{N/2}-1} x(2m+1)W^{km}_{N/2} \label{eq:3.1.8}
\end{align}

On comparing the above equation with the DFT equation \eqref{eq:3dftx}, we can observe that the first term is a N/2-point DFT of $x(2m)$ and second term is a N/2-point DFT of $x(2m+1)$. \\
Let,
\begin{align}
    X_{e}(k) &= \sum_{m=0}^{{N/2}-1} x(2m)W^{km}_{N/2} \\
    &={ F_{N/2}}.x(2m) \\
    X_{o}(k) &= \sum_{m=0}^{{N/2}-1} x(2m+1)W^{km}_{N/2} \\
    &= {F_{N/2}}.x(2m+1)
\end{align}

So, $X(k)$ can be written as,
\begin{align}
    X(k) = X_{e}(k) + W_{N}^k X_{o}(k) \label{eq:3.1.13}
\end{align}
\begin{align}
    F_{N}.x(n) = F_{N/2}.x(2m) + F_{N/2}.x(2m+1) 
\end{align}
From the above equation we can say see that a N-point DFT is calculated from the sum of two N/2-point DFT.

\bigskip
Due to the periodicity of complex exponential function, $W_{N/2}^{nk}$ satisfies the following properties,

\begin{align}
  (ii) \quad W^{k+N/2}_{N/2} = W^{k}_{N/2}
\end{align}
\begin{align}
    \because e^{-j2\pi n(k+N/2)/(N/2)} &= e^{-j2\pi nk/(N/2)}.e^{-j2\pi n} \\
    &= e^{-j2\pi nk/(N/2)}.1 \\
    &= e^{-j2\pi nk/(N/2)}
\end{align}
\begin{align}
  (iii)\quad  W^{k+N/2}_{N} = -W^{k}_{N}\end{align}
\begin{align}
    \because e^{-j2\pi n(k+N/2)/N} &= e^{-j2\pi nk/N}.e^{-j\pi n} \\
    &= e^{-j2\pi nk/N}.(-1) \\
    &= -e^{-j2\pi nk/N}
\end{align}

\newpage
From eq(\eqref{eq:3.1.8}),
\begin{align}
    X(k+N/2) &= \sum_{m=0}^{{N/2}-1} x(2m)W^{m(k+N/2)}_{N/2} +W^{k+N/2}_{N} \sum_{m=0}^{{N/2}-1} x(2m+1)W^{m(k+N/2)}_{N/2}
\end{align}

Using properties (ii) and (iii), we have,
\begin{align}
    X(k+N/2) &= \sum_{m=0}^{{N/2}-1} x(2m)W^{mk}_{N/2} - W^{k}_{N} \sum_{m=0}^{{N/2}-1} x(2m+1)W^{mk}_{N/2} 
\end{align}
\begin{align}
    X(k+N/2) = X_{e}(k) - W_{N}^k X_{o}(k) \label{eq:3.1.25}
\end{align}

Now, from equations \eqref{eq:3.1.13} and \eqref{eq:3.1.25} i.e,
\begin{align}
    X(k) = X_{e}(k) + W_{N}^k X_{o}(k) \\
    X(k+N/2) = X_{e}(k) - W_{N}^k X_{o}(k) 
\end{align}

we have,
\begin{equation}
\begin{bmatrix}
X(0) \\
X(1) \\
X(2) \\
\vdots \\

X(N/2-1)
\end{bmatrix}
= 
\begin{bmatrix}
X_{e}(0) \\
X_{e}(1) \\
X_{e}(2) \\
\vdots \\

X_{e}(N/2-1)
\end{bmatrix}
+
\begin{bmatrix}
W^{0}_{N} & 0  &0 &. &. \\
0 & W^{1}_{N} & 0 & 0 &. \\
0 & 0 & W^{2}_{N} & 0 &. \\
\vdots & \vdots& & \ddots & \vdots\\
0 & 0 &. &. &W^{N/2-1}_{N}
\end{bmatrix}
\begin{bmatrix}
X_{o}(0) \\
X_{o}(1) \\
X_{o}(2) \\
\vdots \\

X_{o}(N/2-1)
\end{bmatrix}
\end{equation}
\bigskip
\begin{equation}
\begin{bmatrix}
X(N/2) \\
X(N/2+1) \\
X(N/2+2) \\
\vdots \\

X(N)
\end{bmatrix}
= 
\begin{bmatrix}
X_{e}(0) \\
X_{e}(1) \\
X_{e}(2) \\
\vdots \\

X_{e}(N/2-1)
\end{bmatrix}
-
\begin{bmatrix}
W^{0}_{N} & 0  &0 &. &. \\
0 & W^{1}_{N} & 0 & 0 &. \\
0 & 0 & W^{2}_{N} & 0 &. \\
\vdots & \vdots& & \ddots & \vdots\\
0 & 0 &. &. &W^{N/2-1}_{N}
\end{bmatrix}
\begin{bmatrix}
X_{o}(0) \\
X_{o}(1) \\
X_{o}(2) \\
\vdots \\
X_{o}(N/2-1)
\end{bmatrix}
\end{equation}

In this way, by dividing the input signal into even and odd indices of n and using the properties of complex exponential we can calculate a N-point DFT by the sum of two N/2-point DFT's. Recursively we can further divide each N/2-point DFT into two N/4-point DFT's and so on. \\
The {\bf{FFT algorithm}} decreases the time complexity from $O(N^{2})$ to $O(NlogN)$, i.e, the DFT is computed faster. \\

\emph{Note: This algorithm is valid only when $N = 2^{m}$ for $m \in \mathbb{Z^{+}}$ is satisfied}

%%%%%%%%%%%%%%%%%%%%%%%%%%%%%%%%%%%%%%%%%%%%%%%-- 8-point FFT
\newpage
.
\newpage
\item
{\bf{FFT algorithm for 8-point DFT:}}

For a signal x(n) and $N=8(=2^{3})$,\\
The 8-point DFT is given by,
\begin{align}
  X(k) = F_{8}.x(n)
\end{align}
Using the FFT algorithm we can write 8-point DFT in 4-point DFT's,
\begin{equation}
\begin{bmatrix}
X(0) \\ 
X(1) \\ 
X(2) \\ 
X(3)
\end{bmatrix}
=
\begin{bmatrix}
X_{e}(0) \\ 
X_{e}(1)\\ 
X_{e}(2)\\
X_{e}(3)\\
\end{bmatrix}
+
\begin{bmatrix}
W^{0}_{8} & 0 & 0 & 0\\
0 & W^{1}_{8} & 0 & 0\\
0 & 0 & W^{2}_{8} & 0\\
0 & 0 & 0 & W^{3}_{8}
\end{bmatrix}
\begin{bmatrix}
X_{o}(0) \\ 
X_{o}(1) \\ 
X_{o}(2) \\
X_{o}(3)
\end{bmatrix}
\end{equation}
\begin{equation}
\begin{bmatrix}
X(4) \\ 
X(5) \\ 
X(6) \\ 
X(7)
\end{bmatrix}
=
\begin{bmatrix}
X_{e}(0) \\ 
X_{e}(1)\\ 
X_{e}(2)\\
X_{e}(3)\\
\end{bmatrix}
-
\begin{bmatrix}
W^{0}_{8} & 0 & 0 & 0\\
0 & W^{1}_{8} & 0 & 0\\
0 & 0 & W^{2}_{8} & 0\\
0 & 0 & 0 & W^{3}_{8}
\end{bmatrix}
\begin{bmatrix}
X_{o}(0) \\ 
X_{o}(1) \\ 
X_{o}(2) \\
X_{o}(3)
\end{bmatrix}
\end{equation}

Here, 
\begin{align}
    X_{e} = F_{4}.[x(0),x(2),x(4),x(6)] \\
    X_{o} = F_{4}.[x(1),x(3),x(5),x(7)]
\end{align}
Now, from 4-point DFT's we get 2-point DFT's recursively,
\begin{equation}
\begin{bmatrix}
X_{e}(0) \\ 
X_{e}(1)\\ 
\end{bmatrix}
=
\begin{bmatrix}
X_{ee}(0) \\ 
X_{ee}(1)\\ 
\end{bmatrix}
+
\begin{bmatrix}
W^{0}_{4} & 0\\
0 & W^{1}_{4}
\end{bmatrix}
\begin{bmatrix}
X_{eo}(0) \\ 
X_{eo}(1) \\ 
\end{bmatrix}
\end{equation}
\begin{equation}
\begin{bmatrix}
X_{e}(2) \\ 
X_{e}(3)\\ 
\end{bmatrix}
=
\begin{bmatrix}
X_{ee}(0) \\ 
X_{ee}(1)\\ 
\end{bmatrix}
-
\begin{bmatrix}
W^{0}_{4} & 0\\
0 & W^{1}_{4}
\end{bmatrix}
\begin{bmatrix}
X_{eo}(0) \\ 
X_{eo}(1) \\ 
\end{bmatrix}
\end{equation}
\begin{equation}
\begin{bmatrix}
X_{o}(0) \\ 
X_{o}(1)\\ 
\end{bmatrix}
=
\begin{bmatrix}
X_{oe}(0) \\ 
X_{oe}(1)\\ 
\end{bmatrix}
+
\begin{bmatrix}
W^{0}_{4} & 0\\
0 & W^{1}_{4}
\end{bmatrix}
\begin{bmatrix}
X_{oo}(0) \\ 
X_{oo}(1) \\ 
\end{bmatrix}
\end{equation}
\begin{equation}
\begin{bmatrix}
X_{o}(2) \\ 
X_{o}(3)\\ 
\end{bmatrix}
=
\begin{bmatrix}
X_{oe}(0) \\ 
X_{oe}(1)\\ 
\end{bmatrix}
-
\begin{bmatrix}
W^{0}_{4} & 0\\
0 & W^{1}_{4}
\end{bmatrix}
\begin{bmatrix}
X_{oo}(0) \\ 
X_{oo}(1) \\ 
\end{bmatrix}
\end{equation}

Here,
\begin{align}
    X_{ee} &= [X_{e}(0),X_{e}(2)] \\
    &=F_{2}.[x(0),x(4)]\\
    X_{eo} &= [X_{e}(1),X_{e}(3)]\\
    &=F_{2}.[x(2),x(6)]\\
    X_{oe} &= [X_{o}(0),X_{o}(2)] \\
    &=F_{2}.[x(1),x(5)]\\
    X_{oo} &= [X_{o}(1),X_{o}(3)]\\
    &=F_{2}.[x(3),x(7)]
\end{align}

\newpage
Now, 2-point DFT Matrix is given by, 

\begin{equation}
\because
F_{2} =
\begin{bmatrix}
1 & 1 \\
1&-1
\end{bmatrix}
\end{equation}

$\implies$ we get,
\begin{equation}
\begin{bmatrix}
X_{ee}(0) \\ 
X_{ee}(1)\\ 
\end{bmatrix}
= F_{2}
\begin{bmatrix}
x(0) \\ 
x(4) \\ 
\end{bmatrix}
=
\begin{bmatrix}
x(0)+x(4) \\ 
x(0)-x(4) \\ 
\end{bmatrix}
\end{equation}
\begin{equation}
\begin{bmatrix}
X_{eo}(0) \\ 
X_{eo}(1)\\ 
\end{bmatrix}
= F_{2}
\begin{bmatrix}
x(2) \\ 
x(6) \\ 
\end{bmatrix}
=
\begin{bmatrix}
x(2)+x(6) \\ 
x(2)-x(6) \\ 
\end{bmatrix}
\end{equation}
\begin{equation}
\begin{bmatrix}
X_{oe}(0) \\ 
X_{oe}(1)\\ 
\end{bmatrix}
= F_{2}
\begin{bmatrix}
x(1) \\ 
x(5) \\ 
\end{bmatrix}
=
\begin{bmatrix}
x(1)+x(5) \\ 
x(1)-x(5) \\ 
\end{bmatrix}
\end{equation}
\begin{equation}
\begin{bmatrix}
X_{oo}(0) \\ 
X_{oo}(1)\\ 
\end{bmatrix}
= F_{2}
\begin{bmatrix}
x(3) \\ 
x(7) \\ 
\end{bmatrix}
=
\begin{bmatrix}
x(3)+x(7) \\ 
x(3)-x(7) \\ 
\end{bmatrix}
\end{equation}
\bigskip
\item
{\bf{Example problem:}}

Let x(n) be a input signal,
\begin{align}
    x(n) = \cbrak{\underset{\uparrow}{1},2,3,4,2,1} 
\end{align}

Now to compute 8-point DFT, N should be 8. \\
$\because$ For input signal N=6.\\
So for N=8 we zero-pad the input signal with 2 zeros.\\
\begin{align}
    \implies x(n) = \cbrak{\underset{\uparrow}{1},2,3,4,2,1,0,0} 
\end{align}

The 8-point FFT algorithm to compute the fourier transform of x(n) and h(n)is in the following python code.
\begin{lstlisting}
https://github.com/pranayEE11009/EE3025_IDP/blob/main/Assignment_1/codes/ee18btech11009_fft.py
\end{lstlisting}

\bigskip
The following C program computes the 8-point FFT.
\begin{lstlisting}
https://github.com/pranayEE11009/EE3025_IDP/blob/main/Assignment_1/codes/ee18btech11009_fft.c
\end{lstlisting}
%%%%%%%%%%%%%%%%%%%%%%%%%%%%%%%%%%%%%%%%%%%%%%%%%%%%%%%%%%%
\newpage

\begin{figure}[h!]
    \centering
    \includegraphics[height=6.8cm,width=9cm]{x_fft.png}
    \label{figs}
\end{figure}

\begin{figure}[h!]
    \centering
    \includegraphics[height=6.8cm,width=9cm]{Xamp_fft.png}
    \label{figs}
\end{figure}

\begin{figure}[h!]
    \centering
    \includegraphics[height=6.8cm,width=9.25cm]{Hamp_fft.png}
    \label{figs}
\end{figure}

\begin{figure}[h!]
    \centering
    \includegraphics[height=6.8cm,width=9cm]{h_fft.png}
    \label{figs}
\end{figure}
\vspace{1cm}
\begin{figure}[h!]
    \centering
    \includegraphics[height=6.8cm,width=9.5cm]{Xpha_fft.png}
    \label{figs}
\end{figure}

\begin{figure}[h!]
    \centering
    \includegraphics[height=6.8cm,width=9.5cm]{Hpha_fft.png}
    \label{figs}
\end{figure}
\end{enumerate}
\end{document}